{
 "cells": [
  {
   "cell_type": "markdown",
   "metadata": {},
   "source": [
    "# Homework 6\n",
    "\n",
    "## Readings: Lecture 07"
   ]
  },
  {
   "cell_type": "markdown",
   "metadata": {},
   "source": [
    "## Problem 1\n",
    "\n",
    "For $f\\in C^1(\\mathbb{R}^n)$ and $\\gamma\\in C^1(\\mathbb{R};\\mathbb{R}^n)$, the multivariate Taylor's theorem gives us a $\\tau\\in (t, t+h)$ such that \n",
    "\n",
    "$$\n",
    "\\gamma(t+h)=\\gamma(t) + \\frac{d\\gamma}{dt}(\\tau)h,\n",
    "$$\n",
    "\n",
    "and a $\\nu$ between $\\gamma(t)$ and $\\gamma(t) + \\frac{d\\gamma}{dt}(\\tau)h$ such that\n",
    "\n",
    "$$\n",
    "\\begin{align}\n",
    "f(\\gamma(t+h))=&f\\left(\\gamma(t) + \\frac{d\\gamma}{dt}(\\tau)h\\right)\\\\\n",
    "=&f(\\gamma(t))+\\nabla f(\\nu)^T\\frac{d\\gamma}{dt}(\\tau)h.\n",
    "\\end{align},\n",
    "$$\n",
    "\n",
    "Therefore,\n",
    "\n",
    "$$\n",
    "\\frac{f(\\gamma(t+h))-f(\\gamma(t))}{h} =\\frac{\\nabla f(\\nu)^T\\frac{d\\gamma}{dt}(\\tau)h}{h}=\\nabla f(\\nu)^T\\frac{d\\gamma}{dt}(\\tau)\n",
    "$$\n",
    "\n",
    "for any $h\\not=0$. As $h\\rightarrow 0$, $\\tau\\rightarrow t$, and $\\nu\\rightarrow \\gamma(t)$. Consequently, the limit of this difference quotient is $\\nabla f(\\gamma(t))^T\\frac{d\\gamma}{dt}(t)$, and the first **multivariate chain rule** is\n",
    "\n",
    "$$\n",
    "\\frac{d}{dt} f(\\gamma(t)) = \\nabla f(\\gamma(t))^T\\frac{d\\gamma}{dt}(t)\n",
    "$$\n",
    "\n",
    "### Part A\n",
    "\n",
    "If $g\\in C^1(\\mathbb{R}^m)$ and $f\\in C^1(\\mathbb{R}^n;\\mathbb{R}^m)$, then $g\\circ f:\\mathbb{R}^n\\rightarrow\\mathbb{R}$ is in $C^1(\\mathbb{R}^n)$. Prove the **chain rule**:\n",
    "\n",
    "$$\n",
    "\\nabla(g\\circ f)({\\bf x}) = Df({\\bf x})^T\\nabla g(f({\\bf x})).\n",
    "$$\n",
    "\n",
    "\n",
    "### Part B\n",
    "If $g\\in C^1(\\mathbb{R}^k;\\mathbb{R}^m)$ and $f\\in C^1(\\mathbb{R}^n;\\mathbb{R}^k)$, then $g\\circ f\\in C^1(\\mathbb{R}^n; \\mathbb{R}^m)$. Prove the **chain rule**:\n",
    "\n",
    "$$\n",
    "D(g\\circ f)({\\bf x}) = Dg(f({\\bf x}))Df({\\bf x}).\n",
    "$$\n"
   ]
  },
  {
   "cell_type": "markdown",
   "metadata": {},
   "source": [
    "## Solution to Problem 1\n",
    "### Part A\n",
    "$$\\nabla(g \\circ f)({\\bf x})=\\begin{pmatrix}\n",
    "\\frac{\\partial(g \\circ f)}{\\partial x_1}(x)\\\\\n",
    "\\vdots\\\\\n",
    "\\frac{\\partial(g \\circ f)}{\\partial x_n}(x)\n",
    "\\end{pmatrix}$$\n",
    "$$=\\begin{pmatrix}\n",
    "\\nabla g(f(x))^T \\frac{\\partial f}{\\partial x_1}(x)\\\\\n",
    "\\vdots\\\\\n",
    "\\nabla g(f(x))^T \\frac{\\partial f}{\\partial x_n}(x)\n",
    "\\end{pmatrix}$$\n",
    "$$= Df({\\bf x})^T\\nabla g(f({\\bf x}))$$\n",
    "### Part B\n",
    "We write $g(y)$ as:\n",
    "$$g(y)=\\begin{pmatrix}\n",
    "g_1(y)\\\\\n",
    "\\vdots\\\\\n",
    "g_m(y)\n",
    "\\end{pmatrix}$$\n",
    "in which $g_i(y)\\in C^1(\\mathbb{R}^k;\\mathbb{R})$\n",
    "Then:\n",
    "$$D(g \\circ f)(\\bf x)=\\begin{pmatrix}\n",
    "\\nabla(g_1 \\circ f)(\\bf x)^T)\\\\\n",
    "\\vdots\\\\\n",
    "\\nabla(g_m \\circ f)(\\bf x)^T)\n",
    "\\end{pmatrix}$$\n",
    "$$=\\begin{pmatrix}\n",
    "\\nabla g_1(f({\\bf x}))^TDf(\\bf x)\\\\\n",
    "\\vdots\\\\\n",
    "\\nabla g_m(f({\\bf x}))^TDf(\\bf x)\n",
    "\\end{pmatrix}$$\n",
    "$$=\\begin{pmatrix}\n",
    "\\nabla g_1(f({\\bf x}))^T\\\\\n",
    "\\vdots\\\\\n",
    "\\nabla g_m(f({\\bf x}))^T\n",
    "\\end{pmatrix}Df({\\bf x})$$\n",
    "$$=Dg(f({\\bf x}))Df({\\bf x})$$"
   ]
  },
  {
   "cell_type": "markdown",
   "metadata": {},
   "source": [
    "## Problem 2\n",
    "\n",
    "Suppose $y\\in\\mathbb{R}^N$, $X\\in\\mathbb{R}^{N\\times(d+1)}$, and define $f:\\mathbb{R}^{d+1}\\rightarrow\\mathbb{R}^N$ and $g:\\mathbb{R}^N\\rightarrow\\mathbb{R}$ by \n",
    "\n",
    "$$\n",
    "f(\\beta)=X\\beta-y\\text{ and } g(x)=\\frac{1}{2}\\Vert x\\Vert^2\n",
    "$$\n",
    "\n",
    "Compute $Df(\\beta)$, $\\nabla g(x)$, and use the chain rule to compute $\\nabla (g\\circ f)(\\beta)=\\nabla\\left[\\frac{1}{2}\\Vert y-X\\beta\\Vert^2\\right]$.\n"
   ]
  },
  {
   "cell_type": "markdown",
   "metadata": {},
   "source": [
    "## Solution to Problem 2\n",
    "We write $f(\\beta)$ as:\n",
    "$$\\begin{pmatrix}\n",
    "\\alpha_1\\\\\n",
    "\\vdots\\\\\n",
    "\\alpha_N\n",
    "\\end{pmatrix}$$\n",
    "We write elements of $X$ as $\\{x_{i,j};i=1,...,N;j=1,...,d+1\\}$\n",
    "We write $\\beta$ as:\n",
    "$$\\begin{pmatrix}\n",
    "\\beta_1\\\\\n",
    "\\vdots\\\\\n",
    "\\beta_{d+1}\n",
    "\\end{pmatrix}$$\n",
    "We compute $X\\beta$. Then we have:\n",
    "$$X\\beta=\\begin{pmatrix}\n",
    "\\sum_{j=1}^{d+1}x_{1,j}\\beta_j\\\\\n",
    "\\vdots\\\\\n",
    "\\sum_{j=1}^{d+1}x_{i,j}\\beta_j\\\\\n",
    "\\vdots\\\\\n",
    "\\sum_{j=1}^{d+1}x_{N,j}\\beta_j\n",
    "\\end{pmatrix}$$\n",
    "Then we compute $D(f\\beta)$:\n",
    "$$D(f(\\beta))=D(X\\beta)$$\n",
    "$$=\\begin{pmatrix}\n",
    "x_{1,1}&\\cdots&x_{1,d+1}\\\\\n",
    "x_{2,1}&\\cdots&x_{2,d+1}\\\\\n",
    "\\vdots&\\vdots&\\vdots\\\\\n",
    "x_{N,1}&\\cdots&x_{N,d+1}\n",
    "\\end{pmatrix}$$\n",
    "$$=X$$\n",
    "Then we compute $\\nabla g(x)$:\n",
    "$$g(x)=\\frac{1}{2}(x_1^2+x_2^2+\\cdots+x_N^2)$$\n",
    "$$\\frac{\\partial g(x)}{\\partial x_i}=x_i,i=1,\\cdots,N$$\n",
    "That is:\n",
    "$$\\nabla g(x)=\\begin{pmatrix}\n",
    "x_1\\\\\n",
    "\\vdots\\\\\n",
    "x_N\n",
    "\\end{pmatrix}$$\n",
    "$$=x$$\n",
    "$$\\nabla(g\\circ f)({\\beta}) = Df({\\beta})^T\\nabla g(f({\\beta}))$$\n",
    "$$=X^T(X\\beta-y)$$\n",
    "$$=X^TX\\beta-X^Ty$$"
   ]
  },
  {
   "cell_type": "markdown",
   "metadata": {},
   "source": [
    "## Problem 3\n",
    "\n",
    "Given $v\\in\\mathbb{R}^d$, let $f(x)=\\frac{1}{2}\\Vert x-v\\Vert^2+\\sum_{i=1}^d\\vert x_i\\vert$. Show that $f$ is strictly convex, and find the unique minimizer $x^\\ast$ of $f$ over $\\mathbb{R}^d$."
   ]
  },
  {
   "cell_type": "markdown",
   "metadata": {},
   "source": [
    "## Solution to Problem 3\n",
    "We let $g(x)=\\frac{1}{2}\\Vert x-v\\Vert^2$ and $h(x)=\\sum_{i=1}^d\\vert x_i\\vert$\n",
    "$$\\frac{\\partial^2 g(x)}{\\partial x_i\\partial x_j}=\n",
    "\\begin{cases}\n",
    "1&when\\ i=j\\\\\n",
    "0&when\\ i\\neq j\n",
    "\\end{cases}$$\n",
    "So $\\nabla^2g(x)$ is an identity matrix, which is surely positive definite. That indicates $g(x)$ being strictly convex.  \n",
    "As for $h(x)$, we suppose $x,y\\in R^d$ and $t\\in [0,1]$  \n",
    "Then we have:\n",
    "$$h(tx+(1-t)y)$$\n",
    "$$=\\sum_{i=1}^{d}\\vert tx_i+(1-t)y_i\\vert$$\n",
    "$$\\leq \\sum_{i=1}^{d}(\\vert tx_i\\vert + \\vert(1-t)y_i\\vert)$$\n",
    "$$=t\\sum_{i=1}^{d}\\vert x_i\\vert+(1-t)\\sum_{i=1}^{d}\\vert y_i\\vert$$\n",
    "$$=th(x)+(1-t)h(y)$$\n",
    "That indicates $h(x)$ being convex.  \n",
    "So $f(x)$, the sum of $g(x)$ and $h(x)$, is strictly convex.  \n",
    "\n",
    "We let $$s(q)=\\min_p k(p,q)=\\min_p(\\frac{1}{2}(p-q)^2+\\vert p\\vert)$$\n",
    "$$k(p,q)=\\begin{cases}\n",
    "\\frac{1}{2}(p^2-(2q-2)p+q^2)&when\\ p>0\\\\\n",
    "\\frac{1}{2}(p^2-(2q+2)p+q^2)&when\\ p\\leq0\n",
    "\\end{cases}$$\n",
    "#### (1)\n",
    "When $q<-1$:\n",
    "$$min_{p,p\\geq0}k(p,q)=\\frac{1}{2}q^2$$\n",
    "$$min_{p,p\\leq0}k(p,q)=-q-\\frac{1}{2}$$\n",
    "We have:\n",
    "$$\\frac{1}{2}q^2\\geq-q-\\frac{1}{2}$$\n",
    "So we have:\n",
    "$$s(q)=min_{p}k(p,q)=-q-\\frac{1}{2}\\ (p=q+1)$$\n",
    "\n",
    "#### (2)\n",
    "When $-1\\leq q\\leq1$:\n",
    "$$min_{p,p\\geq0}k(p,q)=\\frac{1}{2}q^2$$\n",
    "$$min_{p,p\\leq0}k(p,q)=\\frac{1}{2}q^2$$\n",
    "So we have:\n",
    "$$s(q)=min_{p}k(p,q)=\\frac{1}{2}q^2\\ (p=0)$$\n",
    "\n",
    "#### (3)\n",
    "When $q>1$:\n",
    "$$min_{p,p\\geq0}k(p,q)=q-\\frac{1}{2}$$\n",
    "$$min_{p,p\\leq0}k(p,q)=\\frac{1}{2}q^2$$\n",
    "We have:\n",
    "$$q-\\frac{1}{2}\\leq \\frac{1}{2}q^2$$\n",
    "So we have:\n",
    "$$s(q)=min_{p}k(p,q)=q-\\frac{1}{2}\\ (p=q-1)$$  \n",
    "  \n",
    "In conclusion:\n",
    "$$s(q)=\\begin{cases}\n",
    "-q-\\frac{1}{2}&when\\ q<-1\\\\\n",
    "\\frac{1}{2}q^2&when\\ -1\\leq q\\leq1\\\\\n",
    "q-\\frac{1}{2}&when\\ q>1\n",
    "\\end{cases}$$\n",
    "And we let $$r(q)=argmin_p k(p,q)=\n",
    "\\begin{cases}\n",
    "q+1&when\\ q<-1\\\\\n",
    "0&when\\ -1\\leq q\\leq1\\\\\n",
    "q-1&when\\ q>1\n",
    "\\end{cases}$$\n",
    "  \n",
    "Back to the problem, we have:\n",
    "$$f(x)=\\sum_{i=1}^{d}k(x_i,v_i)$$\n",
    "$$\\min_xf(x)=\\min_x\\sum_{i=1}^{d}k(x_i,v_i)$$\n",
    "$$=\\sum_{i=1}^{d}\\min_{x_i}k(x_i,v_i),\\text{ (considering the independence of }x_i)$$\n",
    "$$=\\sum_{i=1}^{d}s(v_i)$$\n",
    "$$\\text{with }x^\\ast\\text{ being }\\begin{pmatrix}\n",
    "r(v_1)\\\\\n",
    "\\vdots\\\\\n",
    "r(v_d)\n",
    "\\end{pmatrix}$$"
   ]
  },
  {
   "cell_type": "markdown",
   "metadata": {},
   "source": [
    "## Problem 4\n",
    "\n",
    "$$\n",
    "f(a,b,c) = -\\log\\det\\begin{pmatrix} a & b\\\\b&c\\end{pmatrix}.\n",
    "$$\n",
    "\n",
    "Show that $\\nabla^2 f(a,b,c)$ is positive semidefinite if $a>0$ and $ac-b^2>0$. \n"
   ]
  },
  {
   "cell_type": "markdown",
   "metadata": {},
   "source": [
    "## Solution to Problem 4"
   ]
  },
  {
   "cell_type": "markdown",
   "metadata": {
    "collapsed": true
   },
   "source": [
    "We first compute $f(a,b,c)$:\n",
    "$$f(a,b,c)=-log(ac-b^2)$$\n",
    "We compute $\\nabla f(a,b,c)$:\n",
    "$$\\nabla f(a,b,c)=\\begin{pmatrix}\n",
    "-\\frac{c}{ac-b^2}\\\\\n",
    "\\frac{2b}{ac-b^2}\\\\\n",
    "-\\frac{a}{ac-b^2}\n",
    "\\end{pmatrix}$$\n",
    "Then we compute $\\nabla^2f(a,b,c)$:\n",
    "$$\\nabla^2f(a,b,c)=\\begin{pmatrix}\n",
    "\\frac{c^2}{(ac-b^2)^2}&-\\frac{2bc}{(ac-b^2)^2}&\\frac{b^2}{(ac-b^2)^2}\\\\\n",
    "-\\frac{2bc}{(ac-b^2)^2}&\\frac{2ac+2b^2}{(ac-b^2)^2}&-\\frac{2ab}{(ac-b^2)^2}\\\\\n",
    "\\frac{b^2}{(ac-b^2)^2}&-\\frac{2ab}{(ac-b^2)^2}&\\frac{a^2}{(ac-b^2)^2}\n",
    "\\end{pmatrix}$$\n",
    "$$=\\frac{1}{(ac-b^2)^2}\\begin{pmatrix}\n",
    "c^2&-2bc&b^2\\\\\n",
    "-2bc&2ac+2b^2&-2ab\\\\\n",
    "b^2&-2ab&a^2\n",
    "\\end{pmatrix}$$\n",
    "We have:\n",
    "$$det(c^2)\\geq 0$$\n",
    "$$det\\begin{pmatrix}\n",
    "c^2&-2bc\\\\\n",
    "-2bc&2ac+2b^2\n",
    "\\end{pmatrix}=2c^2(ac-b^2)\\geq0$$\n",
    "$$det\\begin{pmatrix}\n",
    "c^2&-2bc&b^2\\\\\n",
    "-2bc&2ac+2b^2&-2ab\\\\\n",
    "b^2&-2ab&a^2\n",
    "\\end{pmatrix}=(2a^2c^2+2b^4-4ab^2c)(ac-b^2)=2(ac-b^2)^2(ac-b^2)\\geq0$$\n",
    "So that indicates $\\nabla^2f(a,b,c)$ is positive semidefinite."
   ]
  }
 ],
 "metadata": {
  "kernelspec": {
   "display_name": "Python 3",
   "language": "python",
   "name": "python3"
  },
  "language_info": {
   "codemirror_mode": {
    "name": "ipython",
    "version": 3
   },
   "file_extension": ".py",
   "mimetype": "text/x-python",
   "name": "python",
   "nbconvert_exporter": "python",
   "pygments_lexer": "ipython3",
   "version": "3.9.0"
  }
 },
 "nbformat": 4,
 "nbformat_minor": 2
}
